Clean/Gadgets/BLAKE3/Round.lean
@@ -104,7 +104,7 @@ def circuit : FormalCircuit (F p) Inputs BLAKE3State := {
     refine ⟨⟨fun h => ?_, fun h => ?_, fun h => ?_, fun h => ?_, fun h => ?_, fun h => ?_,
              fun h => ?_, fun h => ?_⟩, fun h h_agrees => ?_⟩
     · exact FormalCircuit.toSubcircuit_computableWitnesses_onlyAccessedBelow_of_offset_eq _
-        (by first | omega | (simp only [eG]; try omega)) fun h_agrees => by
+        (by omega) fun h_agrees => by
           simp only [circuit_norm]
           refine ⟨?_, ?_, ?_⟩
           · exact h.1
