Clean/Gadgets/SHA256/UpperSigma0.lean
@@ -214,7 +214,7 @@ def circuit : FormalCircuit (F p) (fields 32) (fields 32) where
   main; elaborated; Assumptions; Spec; soundness; completeness
   computableWitnesses := by
     intro n input env env'
-    simp only [circuit_norm, main, upperSigma0, xor32, rotr32, shr32, Vector.ext_iff]
+    simp only [circuit_norm, main, upperSigma0, xor32, rotr32, Vector.ext_iff]
     refine ⟨⟨fun h hag => ?_, fun h hag => ?_, ?_⟩, fun h hag => ?_⟩
     · intro i hi
       simp only [circuit_norm, Vector.getElem_rotate]
